Tweak a call of COMMENT in prover output pertaining to unknown warrants.
Thanks to J for pointing out and discussing this issue.

The last example in :doc comment showed this:

    (IMPLIES
     (NOT (APPLY$-WARRANT-BAR))
     (EQUAL (HIDE (COMMENT "Call failed because the warrant for BAR is false"
                           (EV$ '(BAR Y) '((Y . 3)))))
            3))

That was correct, but in general the warrant in such a case is merely
unknown, not necessarily false.  That can happen when forcing is
disabled (otherwise the warrant would be assumed true by forcing it).

So now that checkpoint looks as follows:

    (IMPLIES
     (NOT (APPLY$-WARRANT-BAR))
     (EQUAL (HIDE (COMMENT "Call failed because the warrant for BAR is not known to be true"
                           (EV$ '(BAR Y) '((Y . 3)))))
            3))

Additional explanation has been added to :doc comment.

books/system/doc/acl2-doc.lisp
@@ -14997,7 +14997,7 @@ with any questions about building the community books.</p>")
   YYY)
  })
 
- <h3>Evaluation during building a term</h3>
+ <h3>Failure to expand using a rule</h3>
 
  <p>Form:</p>
 
@@ -15017,7 +15017,7 @@ with any questions about building the community books.</p>")
  })
 
  <p>The checkpoint is as follows.  What happened is that the rule @('nth-open')
- had a hypothesis that was false when the rule's was attempted for the term
+ had a hypothesis that was false when the rule was attempted for the term
  @('(nth i y)').</p>
 
  @({
@@ -15027,26 +15027,28 @@ with any questions about building the community books.</p>")
                  ZZZ))
  })
 
- <h3>Failure due to missing or disabled warrants</h3>
+ <h3>Failure due to disabled or missing warrants</h3>
 
  <p>Forms:</p>
 
  @({
  (HIDE (COMMENT \"Call failed because the rule apply$-<fn> is disabled\"
        <term>))
- (HIDE (COMMENT \"Call failed because the warrant for <fn> is false\"
+ (HIDE (COMMENT \"Call failed because the warrant for <fn> is not known to be true\"
        <term>))
  })
 
- <p>These forms may appear when an attempt to evaluate a call of @(tsee apply$)
- fails because a necessary @(see warrant) is either @(see disable)d or known,
- in the present context, to be false.  In the following example, the attempt to
- simplify the call of @('apply$') in the theorem ultimately leads to an attempt
- to evaluate a call of @(tsee ev$), which ultimately fails because it leads to
- a call to evaluate @('(apply$ 'bar '(3))') @('bar').  That call causes an
- error because the warrant is unavailable, because the rule @('apply$-bar') is
- disabled, hence cannot rewrite a term @('(apply$ 'bar args)') to @('(bar (car
- args))').</p>
+ <p>The first of these forms may appear when an attempt to evaluate a call of
+ @(tsee apply$) fails because a necessary @(see warrant) is disable)d.  The
+ second form may appear when the warrant is not known to be true in the present
+ context, either because it is known to be false or because it cannot be
+ assumed true because forcing is @(see disable)d.  In the following example,
+ the attempt to simplify the call of @('apply$') in the theorem ultimately
+ leads to an attempt to evaluate a call of @(tsee ev$), which ultimately fails
+ because it leads to a call to evaluate @('(apply$ 'bar '(3))') @('bar').  That
+ call causes an error because the warrant is unavailable, because the rule
+ @('apply$-bar') is disabled, hence cannot rewrite a term @('(apply$ 'bar
+ args)') to @('(bar (car args))').</p>
 
  @({
  (include-book \"projects/apply/top\" :dir :system)
@@ -15067,7 +15069,7 @@ with any questions about building the community books.</p>")
  })
 
  <p>Similarly, if we instead submit the following event, we see the other such
- message, about a false warrant.</p>
+ message, in this case about a false warrant.</p>
 
  @({
  (thm (implies (not (warrant bar))
@@ -15080,9 +15082,41 @@ with any questions about building the community books.</p>")
  @({
  (IMPLIES
   (NOT (APPLY$-WARRANT-BAR))
-  (EQUAL (HIDE (COMMENT \"Call failed because the warrant for BAR is false\"
+  (EQUAL (HIDE (COMMENT \"Call failed because the warrant for BAR is not known to be true\"
                         (EV$ '(BAR Y) '((Y . 3)))))
          3))
+ })
+
+ <p>Our final example illustrates a failure due to forcing being disabled.  The
+ use of @(tsee loop$) in the definition of @('bar') expands to create a call of
+ @(tsee ev$), which cannot be simplified during the proof of the @(tsee thm)
+ below because the necessary warrant hypothesis is missing and cannot be
+ forced, since forcing is disabled (see also @(see disable-forcing)).</p>
+
+ @({
+ (defun$ hello (x)
+    (declare (xargs :guard t))
+    (list 'hi x))
+
+ (defun bar (lst)
+    (declare (xargs :guard (true-listp lst)))
+    (loop$ for name in lst collect (hello name))))
+
+ (thm (equal (bar '(john))
+             '((hi john)))
+      :hints ((\"Goal\" :in-theory (disable (:e force)))))
+ })
+
+ <p>Here is the resulting checkpoint.</p>
+
+ @({
+ (EQUAL
+  (HIDE
+      (COMMENT
+           \"Call failed because the warrant for HELLO is not known to be true\"
+           (EV$ '(HELLO LOOP$-IVAR)
+                '((LOOP$-IVAR . JOHN)))))
+  '(HI JOHN))
  })")
 
 (defxdoc common-lisp
